Add Mfa Definition (with a few holes)

ProofLibrary/ChaseSequence/Termination/MfaLike.lean
@@ -2,38 +2,219 @@ import ProofLibrary.ChaseSequence.Termination.Basic
 
 variable {sig : Signature} [DecidableEq sig.P] [DecidableEq sig.C] [DecidableEq sig.V]
 
-def criticalInstance (rs : RuleSet sig) (finite : rs.rules.finite) (special_const : sig.C) : Database sig :=
-  ⟨fun f => f.predicate ∈ rs.predicates ∧ ∀ t, t ∈ f.terms -> t = special_const, by
-    have preds_finite := rs.predicates_finite_of_finite finite
-    rcases preds_finite with ⟨l, nodup, eq⟩
-    exists (l.map (fun p => {
-      predicate := p
-      terms := List.repeat special_const (sig.arity p)
-      arity_ok := by rw [List.length_repeat]
-    })).eraseDupsKeepRight
+namespace KnowledgeBase
+
+  def parallelSkolemChase (kb : KnowledgeBase sig) (det : kb.rules.isDeterministic) : InfiniteList (FactSet sig)
+  | .zero => kb.db.toFactSet
+  | .succ n =>
+    let prev_step := parallelSkolemChase kb det n
+    fun f => f ∈ prev_step ∨ (∃ (trg : RTrigger (SkolemObsoleteness sig) kb.rules), trg.val.active prev_step ∧ f ∈ trg.val.result[0]'(by unfold RuleSet.isDeterministic at det; unfold Rule.isDeterministic at det; unfold PreTrigger.result; rw [List.length_map, ← PreTrigger.head_length_eq_mapped_head_length, det trg.val.rule trg.property]; simp))
+
+  theorem parallelSkolemChase_subset_all_following (kb : KnowledgeBase sig) (det : kb.rules.isDeterministic) (n m : Nat) : kb.parallelSkolemChase det n ⊆ kb.parallelSkolemChase det (n+m) := by
+    induction m with
+    | zero => apply Set.subsetOfSelf
+    | succ m ih =>
+      rw [← Nat.add_assoc]
+      conv => right; unfold parallelSkolemChase
+      intro f f_mem
+      apply Or.inl
+      apply ih
+      exact f_mem
+
+  def skolemChaseResult (kb : KnowledgeBase sig) (det : kb.rules.isDeterministic) : FactSet sig := fun f => ∃ n, f ∈ parallelSkolemChase kb det n
+
+  theorem skolemChaseResult_eq_every_chase_branch_result (kb : KnowledgeBase sig) (det : kb.rules.isDeterministic) : ∀ (cb : ChaseBranch (SkolemObsoleteness sig) kb), cb.result = kb.skolemChaseResult det := by
+    unfold RuleSet.isDeterministic at det
+    unfold Rule.isDeterministic at det
+    intro cb
+    apply funext
+    intro f
+    apply propext
+    unfold ChaseBranch.result
+    unfold skolemChaseResult
     constructor
-    . apply List.nodup_eraseDupsKeepRight
-    . intro f
-      rw [List.mem_eraseDupsKeepRight_iff]
-      simp [Set.element]
+    . intro h
+      rcases h with ⟨n, h⟩
+      induction n generalizing f with
+      | zero =>
+        rw [cb.database_first, Option.is_some_and] at h
+        exists 0
+      | succ n ih =>
+        -- should be easy enough: get n from induction hypothesis and then use n+1
+        cases eq_node : cb.branch.infinite_list (n+1) with
+        | none => rw [eq_node, Option.is_some_and] at h; simp at h
+        | some node =>
+          cases eq_prev : cb.branch.infinite_list n with
+          | none => have no_holes := cb.branch.no_holes (n+1); simp [eq_node] at no_holes; specialize no_holes ⟨n, by simp⟩; apply False.elim; apply no_holes; exact eq_prev
+          | some prev_node =>
+            have trg_ex := cb.triggers_exist n
+            rw [eq_prev, Option.is_none_or] at trg_ex
+            cases trg_ex with
+            | inr trg_ex => unfold not_exists_trigger_opt_fs at trg_ex; rw [trg_ex.right] at eq_node; simp at eq_node
+            | inl trg_ex =>
+              unfold exists_trigger_opt_fs at trg_ex
+              rcases trg_ex with ⟨trg, trg_active, disj_index, step_eq⟩
+              rw [← step_eq, Option.is_some_and] at h
+              simp at h
+              cases h with
+              | inl h =>
+                specialize ih f
+                rw [eq_prev, Option.is_some_and] at ih
+                specialize ih h
+                exact ih
+              | inr h =>
+                have : ∃ n, prev_node.fact.val ⊆ kb.parallelSkolemChase det n := by
+                  have prev_finite := prev_node.fact.property
+                  rcases prev_finite with ⟨prev_l, _, prev_l_eq⟩
+
+                  have : ∀ (l : List (Fact sig)), (∀ e, e ∈ l -> e ∈  prev_node.fact.val) -> ∃ n, (∀ e, e ∈ l -> e ∈ kb.parallelSkolemChase det n) := by
+                    intro l l_sub
+                    induction l with
+                    | nil => exists 0; intro e; simp
+                    | cons hd tl ih_inner =>
+                      have from_ih := ih_inner (by intro e e_mem; apply l_sub; simp [e_mem])
+                      rcases from_ih with ⟨n_from_ih, from_ih⟩
+
+                      have from_hd := ih hd
+                      rw [eq_prev, Option.is_some_and] at from_hd
+                      specialize from_hd (by apply l_sub; simp)
+                      rcases from_hd with ⟨n_from_hd, from_hd⟩
+
+                      cases Decidable.em (n_from_ih ≤ n_from_hd) with
+                      | inl le =>
+                        exists n_from_hd
+                        intro f f_mem
+                        simp at f_mem
+                        cases f_mem with
+                        | inl f_mem => rw [f_mem]; exact from_hd
+                        | inr f_mem =>
+                          rcases Nat.exists_eq_add_of_le le with ⟨diff, le⟩
+                          rw [le]
+                          apply kb.parallelSkolemChase_subset_all_following det n_from_ih diff
+                          apply from_ih; exact f_mem
+                      | inr lt =>
+                        simp at lt
+                        have le := Nat.le_of_lt lt
+                        exists n_from_ih
+                        intro f f_mem
+                        simp at f_mem
+                        cases f_mem with
+                        | inr f_mem => apply from_ih; exact f_mem
+                        | inl f_mem =>
+                          rcases Nat.exists_eq_add_of_le le with ⟨diff, le⟩
+                          rw [le]
+                          apply kb.parallelSkolemChase_subset_all_following det n_from_hd diff
+                          rw [f_mem]; exact from_hd
+
+                  specialize this prev_l (by intro f; exact (prev_l_eq f).mp)
+                  rcases this with ⟨n, this⟩
+                  exists n
+                  intro f
+                  rw [← prev_l_eq]
+                  exact this f
+                rcases this with ⟨n, prev_subs⟩
+
+                exists n+1
+                unfold parallelSkolemChase
+
+                have disj_index_zero : disj_index.val = 0 := by
+                  have isLt := disj_index.isLt
+                  unfold PreTrigger.result at isLt
+                  simp only [List.length_map] at isLt
+                  rw [← PreTrigger.head_length_eq_mapped_head_length] at isLt
+                  rw [det _ trg.property, Nat.lt_one_iff] at isLt
+                  exact isLt
+
+
+                -- TODO: would be Decidable if we define sets in the parallelSkolemChase to be finite
+                cases Classical.em (f ∈ kb.parallelSkolemChase det n) with
+                | inl mem => apply Or.inl; exact mem
+                | inr not_mem =>
+                  apply Or.inr
+                  exists trg
+                  constructor
+                  . unfold Trigger.active
+                    constructor
+                    . unfold PreTrigger.loaded
+                      apply Set.subsetTransitive _ prev_node.fact.val _
+                      constructor
+                      . exact trg_active.left
+                      . exact prev_subs
+                    . intro contra
+                      apply not_mem
+                      rcases contra with ⟨i, contra⟩
+                      apply contra
+                      simp only [disj_index_zero] at h
+                      unfold PreTrigger.result at h
+                      rw [List.getElem_map, ← List.inIffInToSet] at h
+                      have : i.val = 0 := by
+                        have isLt := i.isLt
+                        /- unfold PreTrigger.result at isLt -/
+                        /- simp only [List.length_map] at isLt -/
+                        simp only [← PreTrigger.head_length_eq_mapped_head_length] at isLt
+                        rw [det _ trg.property, Nat.lt_one_iff] at isLt
+                        exact isLt
+                      rw [← List.inIffInToSet, List.get_eq_getElem]
+                      simp only [this]
+                      exact h
+                  . simp only [disj_index_zero] at h
+                    exact h
+    . intro h
+      rcases h with ⟨n, h⟩
+      induction n with
+      | zero =>
+        exists 0
+        rw [cb.database_first, Option.is_some_and]
+        exact h
+      | succ n ih =>
+        -- not as "easy" as the other direcition, we need to invoke fairness somehow and likely need to show that only finitely many triggers are active at the same time...
+        sorry
+
+end KnowledgeBase
+
+namespace RuleSet
+
+  def criticalInstance (rs : RuleSet sig) (finite : rs.rules.finite) (special_const : sig.C) : Database sig :=
+    ⟨fun f => f.predicate ∈ rs.predicates ∧ ∀ t, t ∈ f.terms -> t = special_const, by
+      have preds_finite := rs.predicates_finite_of_finite finite
+      rcases preds_finite with ⟨l, nodup, eq⟩
+      exists (l.map (fun p => {
+        predicate := p
+        terms := List.repeat special_const (sig.arity p)
+        arity_ok := by rw [List.length_repeat]
+      })).eraseDupsKeepRight
       constructor
-      . intro h
-        rcases h with ⟨p, p_mem, f_eq⟩
-        rw [← f_eq]
-        rw [eq] at p_mem
+      . apply List.nodup_eraseDupsKeepRight
+      . intro f
+        rw [List.mem_eraseDupsKeepRight_iff]
+        simp [Set.element]
         constructor
-        . exact p_mem
-        . intro t
-          apply List.mem_repeat
-      . intro h
-        exists f.predicate
-        constructor
-        . rw [eq]; exact h.left
-        . rw [FunctionFreeFact.ext_iff]
-          simp
-          rw [List.repeat_eq_iff_all_val]
+        . intro h
+          rcases h with ⟨p, p_mem, f_eq⟩
+          rw [← f_eq]
+          rw [eq] at p_mem
           constructor
-          . exact f.arity_ok
-          . exact h.right
-  ⟩
+          . exact p_mem
+          . intro t
+            apply List.mem_repeat
+        . intro h
+          exists f.predicate
+          constructor
+          . rw [eq]; exact h.left
+          . rw [FunctionFreeFact.ext_iff]
+            simp
+            rw [List.repeat_eq_iff_all_val]
+            constructor
+            . exact f.arity_ok
+            . exact h.right
+    ⟩
+
+  def mfaSet (rs : RuleSet sig) (finite : rs.rules.finite) (det : rs.isDeterministic) (special_const : sig.C) : FactSet sig :=
+    let kb : KnowledgeBase sig := {
+      rules := rs
+      db := criticalInstance rs finite special_const
+    }
+    kb.skolemChaseResult det
+
+end RuleSet
 
